#+TITLE: calculus
#+KEYWORDS: math, calculus
#+OPTIONS: H:3 toc:2 num:3 ^:nil
#+LANGUAGE: zh-CN
#+AUTHOR: ChrisChen
#+EMAIL: ChrisChen3121@gmail.com

* Limits
** Definition
   Let $f(x)$ be defined on an open interval about $x_0$, except possibly at $x_0$ itself.
   We say that the limit of $f(x)$ as $x$ approaches $x_0$ is the number $L$, and write
   $$\lim_{x\to x_0} f(x) = L$$
   if, for every number $\epsilon>0$, there exists a corresponding number $\delta>0$ such that
   $$\forall x \ 0<|x-x_0|<\delta \Longrightarrow |f(x)-L|<\epsilon$$

*** DNF
    $$\mbox{If }\lim_{x\to a+}f(x)\neq \lim_{x\to a-}f(x), \mbox{then }\lim_{x\to a}f(x)\mbox{ DNF}$$

*** Existence
    $$\mbox{If }\lim_{x\to a+}f(x)=\lim_{x\to a-}f(x)=L, \mbox{then } \lim_{x\to a}f(x)=L$$

** Continuity
   To say "$f(x)$ is continuous at $a$"
   - $f(x)$ is defined at $x=a$
   - $\lim_{x\to a}f(x)$ exists
   - $\lim_{x\to a}f(x) = f(a)$

** Laws
   If $\lim_{x\to c}f(x)=L$ and $\lim_{x\to c}g(x)=M$, then
   - Sum rule
     $$\lim_{x\to c}(f(x)+g(x)) = L+M$$

   - Difference rule
     $$\lim_{x\to c}(f(x)-g(x)) = L-M$$

   - Constant Multiple rule
     $$\lim_{x\to c}(k\cdot f(x)) = k\cdot L$$

   - Product rule
     $$\lim_{x\to c}(f(x)\cdot g(x)) = L\cdot M$$

   - Quotient rule
     $$\lim_{x\to c}\frac{f(x)}{g(x)} = \frac{L}{M}, \ M\neq 0$$

   - Root rule

     If $r$ and $s$ are integer, and $s\neq 0$, then:
     $$\lim_{x\to c}f(x)^{\frac{r}{s}}=L^{\frac{r}{s}}$$

** Theorem
*** Intermediate Value Theorem
    If $f$ is a continuous function on a closed interval $[a,\ b]$,
    and if $y_0$ is any value between $f(a)$ and $f(b)$,
    then $y_0=f(c)$ for some $c$ in $[a,\ b]$.

*** The Sandwich Theorem
    If $g(x)\le f(x)\le h(x)$
    and $\lim_{x\to c}g(x) = \lim_{x\to c} h(x) = L$,
    then,
    $$\lim_{x\to c}f(x)=L$$

*** Theorem 2
    If $f(x)\le g(x)$, $\lim_{x\to c}f(x), \lim_{x\to c}g(x)$ exists，

    then $\lim_{x\to c}f(x)\le \lim_{x\to c}g(x)$

** l'Hôpital's rule
   Let $f$ and $g$ be functions differentiable near $a$.

   If $\lim_{x\to a}f(x)=\lim_{x\to a}g(x)= 0\mbox{ or }\pm\infty$ and $\lim_{x\to a}\frac{f^\prime (x)}{g^\prime (x)}$ exists,
   and $g^\prime(x)\neq 0$ for all $x$ near $a$, then
   $$\lim_{x\to a}\frac{f(x)}{g(x)} = L = \lim_{x\to a}\frac{f'(x)}{g'(x)}$$
*** Form transform
    | Form                                   | transform                                  |
    |----------------------------------------+--------------------------------------------|
    | $\frac{0}{0}$, $\frac{\infty}{\infty}$ | l'Hôpital                                  |
    | $0\cdot \infty$                        | $\frac{\infty}{1/0}$, $\frac{0}{1/\infty}$ |
    | $1^\infty$                             | $e^{\infty\cdot \lg(1)}$                    |
    | $\infty^0$                             | $e^{0\cdot \lg(\infty)}$                    |
    | $0^0$                                  | $e^{0\cdot \lg(0)}$                         |
    | $\infty - \infty$                      | $\frac{1/\infty - 1/\infty}{1/\infty^2}$   |
*** Error
    $$\lim_{x\to \infty}\frac{x+\sin x}{x} = \lim_{x\to \infty}\frac{1+\cos x}{1}$$
    The transform does not exist!!!

** $lim_{x\to 0}\frac{sin(x)}{x}=1$

* Derivatives
** Definition
   The derivative of $f$ at the point $x$ is defined to be
   $$f^\prime(x)=\lim_{h \to 0} \frac{f(x+h) - f(x)}{h}$$
   If the *derivative of $f$ exists* at x, we say that the function is *differentiable* at $x$.
   The derivative of $f$ exists means $\lim_{h \to 0} \frac{f(x+h) - f(x)}{h}$ exists.
*** other form
    $$f^\prime(x)=\lim_{x\to a}\frac{f(x)-f(a)}{x-a}$$

*** $f(x+h)\approx f(x) + f'(x)h$ when $h$ approaches 0

*** $\frac{dy}{dx}$ and $dx$
    Think of $dx$ & $dy$ as infinitesimal quantities.
    $$dy = f^\prime(x) dx$$
    - $d(u+v) = du + dv$
    - $d(uv) = (du)v+u(dv)$

** Differentiable
*** Differentiable $\to$ Continuity
    $$f^\prime(x)=\lim_{x\to a}\frac{f(x)-f(a)}{x-a}\ exists$$
$$\begin{align*}
\lim_{x\to a}(f(x)-f(a)) & = \lim_{x\to a}(x-a)\cdot\lim_{x\to a}\frac{f(x)-f(a)}{x-a}\\
& = 0\cdot f^\prime(x) = 0
\end{align*}$$
$$\lim_{x\to a}f(x) = f(a)$$
which means $f(x)$ is continuous at $a$.

*** Continuity $\nrightarrow$ Differentiable
    $f(x) = |x|$ is continuous at 0, but is not differentiable at 0.

** Rules
*** Constant Multiple Rule
    $$\frac{d}{dx}kf(x)=k\frac{d}{dx}f(x)$$

*** Power Rule
    $$\frac{d}{dx}(x^n)=nx^{n-1}$$
**** Proof
$$\begin{align*}
f^\prime(x) & =\lim_{h\to 0}\frac{(x+h)^n-x^n}{h} \\
& = \lim_{h\to 0}\frac{\sum_{k=0}^{n}{n\choose k}x^k h^{n-k}-x^n}{h} \\
& = \lim_{h\to 0}\sum_{k=0}^{n-1}{n\choose k}x^k h^{n-k-1} \\
& = \lim_{h\to 0}({n \choose n-1}x^{n-1}h^0 + \sum_{k=0}^{n-2}{n\choose k}x^k h^{n-k-1}) \\
& = nx^{n-1}
\end{align*}$$
*** Product Rule
    $$\frac{d}{dx}(fg)=f'g + fg'$$
*** Quotient Rule
    $$\frac{d}{dx}(\frac{f}{g})=\frac{f'g-fg'}{g^2}$$
*** Trigonometric Rule
    $$\frac{d}{dx}(\sin x)=\cos x$$
    $$\frac{d}{dx}(\cos x)=-\sin x$$
    $$\frac{d}{dx}(\tan x)=\frac{d}{dx}(\frac{\sin x}{\cos x})=\frac{\cos^2 x+\sin^2 x}{\cos^2 x}=\sec^2 x$$
    $$\frac{d}{dx}(\sec x)=\sec x \tan x$$
    $$\frac{d}{dx}(\cot x)=-\csc^2 x$$
    $$\frac{d}{dx}(\csc x)=-\csc x \cot x$$
    - inverse trigonometric [[https://www.coursera.org/learn/calculus1/lecture/87U1i/what-are-the-derivatives-of-inverse-trig-functions][Proof]]
    $$\frac{d}{dx}(\arcsin x)=\frac{1}{\sqrt{1-x^2}}$$
    $$\frac{d}{dx}(arccsc\ x)=-\frac{1}{|x|\sqrt{x^2-1}}$$
    $$\frac{d}{dx}(\arccos x)=-\frac{1}{\sqrt{1-x^2}}$$
    $$\frac{d}{dx}(arcsec\ x)=\frac{1}{|x|\sqrt{x^2-1}}$$
    $$\frac{d}{dx}(\arctan x)=\frac{1}{1+x^2}$$
    $$\frac{d}{dx}(arccot\ x)=-\frac{1}{1+x^2}$$

*** Chain Rule
**** first form
     $$(f \circ g)^\prime (x) = f^\prime(g(x))g^\prime(x)$$
     means:
     $$\frac{\mbox{change in } f(g(x))}{\mbox{change in } x}=\frac{\mbox{change in } f(g(x))}{\mbox{change in }g(x)}\cdot\frac{\mbox{change in } g(x)}{\mbox{change in }x}$$

**** second form
     Let $u = g(x)$, then $f(g(x))$ turns out to be $f(u)$
     $$\frac{df}{dx}=\frac{df}{du}\frac{du}{dx}$$
     - Example
     $$\frac{d}{dx}(\sqrt{x^3-7x})$$
     Let $f(u) = \sqrt u$ and $u = x^3-7x$
     $$\frac{df}{dx} = \frac{df}{du}\frac{du}{dx} = \frac{3x^2 - 7}{2\sqrt u} = \frac{3x^2 - 7}{2\sqrt{x^3-7x}}$$
*** Derivatives of Inverse Function
    $$f^{-1}\prime(x)=\frac{1}{f^\prime(f^{-1}(x))}$$
    $$\frac{\mathrm{d}y}{\mathrm{d}x} = \frac{1}{\frac{\mathrm{d}x}{\mathrm{d}y}}$$

*** Some Proofs
    [[https://www.coursera.org/learn/calculus1/home/week/6][coursera]] How do I justify the derivative rules?
** Higher derivatives
  #+ATTR_HTML: align="center"
  [[file:../resources/calculus/SecondDerivativeMeaning.png]]

** Some derivatives
*** $\ln x$
    $$f(x) = \ln x, f^{-1}(x) = e^x$$
    $$f\prime(x) = \frac{1}{(f^{-1})\prime(f(x))}=\frac{1}{e^{\ln x}}=\frac{1}{x}$$

*** Use $\log$ to simplify derivatives of high power functions
    Logarithms turn *exponentation* into *multiplication*, and *multiplication* into *addition*.
    eg:
    $$y = \frac{(1+x^2)^5\cdot (1+x^3)^8}{(1+x^4)^7}$$
    $$\ln y = 5\ln(1+x^2) + 8\ln(1+x^3) - 7\ln(1+x^4)$$
    $$\frac{1}{y}\frac{\mathrm{d}y}{\mathrm{d}x}=\frac{5\cdot 2x}{1+x^2} + \frac{8\cdot 3x^2}{1+x^3} - \frac{7\cdot 4x^3}{1+x^4}=\cdots$$

** Application
*** Solving related rates problem
    1. Draw picture
    2. Find equation
    3. Differentiate
    4. Solve
*** Newton's method
    is a method for finding successively better approximations to the *roots (or zeroes)* of a real-valued function.
    [[file:../resources/calculus/Newtonsmethod.png]]
    1. Initial guess $x_0$
    2. New guess $x_1=x_0-\frac{f(x_0)}{f^\prime(x_0)}$
    3. $x_2=x_1-\frac{f(x_1)}{f^\prime(x_1)}$
    4. ...
**** finding root
**** finding zeroes
     find a function $f(\frac{1}{b})=0$:
     - $f(x)=\frac{1}{x}-b$
     - $f^\prime(x)=-\frac{1}{x^2}$

     $$x_{n+1}=x_n-\frac{f(x_n)}{f^\prime(x_n)}=x_n(2-bx_n)$$

** Theorem
*** Extreme value theorem
**** Simple definition
    #+BEGIN_VERSE
    If a function /f/ is continuous on the closed interval [a, b],
    then,
      /f/ attains a maximum value
    and
      /f/ attains a minimum value
    #+END_VERSE

**** Definition
    #+BEGIN_VERSE
    If a function /f/ is continuous on the *closed* interval [a, b],
    then there are $c$ and $d$ in [a, b]
    so that for all x in [a, b],
    $f(c) \le f(x) \le f(d)$
    #+END_VERSE

**** Find extreme value
     1. Differentiate
     2. List critical points, endpoints and non differentiable point
     3. Check those
     4. Check limiting behavior

*** Mean value theorem
**** Concept
     Average velocity is achieved, at some point, instantaneously.

**** Definition
     Suppose $f$ is continuous on $[a, b]$ and differentiable on $(a, b)$, then:

     there exists $c$ in $(a, b)$, so that
     $$f^\prime (c) = \frac{f(b)-f(a)}{b-a}$$

**** Application
     - prove $f(x)$ is constant if $f^\prime(x)=0$ on whole interval
     - prove $f(x)$ is increasing if $f^\prime(x)>0$

* Integration
** Antiderivative
   if $F$ is an antiderivative of $f$, then
   $$\int f(x) dx=F(x)+C$$
** Toolbox
*** $\int\frac{1}{x}dx=ln|x| + C(x)$, $C(x)$ is *locally constant function*
*** $\int f(mx+b)dx=\frac{F(mx+b)}{m}+C$
*** $\int \sin^2 x dx$
    $$\sin^2 x=\frac{1-\cos(2x)}{2}$$
    $$\int \frac{1-\cos(2x)}{2}dx = \frac{x}{2}-\frac{\sin(2x)}{4}+C$$

** Approxmation
*** Riemann Sum
    1. Partition the interval [a, b], $x_0=a < x_1 < x_2 < \cdots < x_n = b$
    2. Choose sample point $x_i^*$

    $$Area \approx \sum_{i=1}^{n}f(x_i^*)\cdot(x_i-x_{i-1})$$
**** Left Riemann Sum $x_i^*=x_{i-1}$
**** Right Riemann Sum $x_i^*=x_i$

** Definition
   $$\int_a^bf(x)dx=\lim_{n\to\infty}\sum_{i=1}^nf(x_i)(x_i-x_{i-1})$$
   $n\to\infty$ *means* partitions max width $\to 0$

** Theorem
*** If $f$ is continuous, then $f$ is integrable
** Rules
*** Constant Multiple Rule
    $$\int kf(x) = k\int f(x)$$

*** Sum Rule
    $$\int(f(x)+g(x))dx=\int f(x)dx + \int g(x)dx=F(x)+G(x)+C$$

*** Power Rule
    $$\int x^n dx=\frac{x^{n+1}}{n+1} + C$$

*** U-Substitution Rule
    - Chain rule in reverse
    let $u=g(x)$, then $du=g'(x)dx$
    $$\int f(g(x))g^\prime(x)dx=\int f(u)du$$
**** e.g. $\int e^\sqrt{x}dx$
     let $u=\sqrt{x}$, then $du=\frac{1}{2\sqrt{x}}dx$, $dx = 2\sqrt{x}du = 2udu$
     $$\int e^\sqrt{x}dx = \int e^u 2udu = \cdots$$

**** e.g. $\int \sin^{odd} xdx$
     $$\int \sin^5 xdx=\int (\sin^2 x)^2 \sin x dx=-\int (1-\cos^2 x)^2 (-\sin x)dx$$
     let $u=\cos x$, then $du=-\sin x dx$
     $$=-\int (1-u^2)^2du=-\int (1-2u^2+u^4)=-u+2\frac{u^3}{3}-\frac{u^5}{5}$$
     $$=-\cos x+2\frac{\cos^3 x}{3}-\frac{\cos^5 x}{5}+C$$

*** Integration By Parts
    - Product rule in reverse
    $$\int f(x)g^\prime(x) dx = f(x)g(x) - \int f^\prime(x)g(x) dx$$
    let $u=f(x)$, $v=g(x)$, then $du=f^\prime(x)dx$, $dv=g^\prime(x)dx$
    $$\int udv = uv - \int vdu$$
**** e.g. $\int xe^x dx$
     pick $u=x,\ dv=e^xdx$

     then $du=dx,\ v=e^x$

     $$\int xe^x dx = xe^x-\int e^x dx$$

     - verify by differentiating result with product rule
** Some Integrations
*** $\int \sin^{even} xdx$
    - Use Half Angle Formula
      $$\sin^2 x=\frac{1-\cos 2x}{2}$$
      $$\cos^2 x=\frac{1+\cos 2x}{2}$$

    $$\int \sin^4 xdx=\int(\sin^2 x)^2 dx=\int(\frac{1-\cos (2x)}{2})^2 dx$$
    $$=\int(\frac{\cos^2(2x)}{4}-\frac{1}{2}\cos(2x)+\frac{1}{4})dx$$
    $$=\int(\frac{1+\cos(4x)}{8}dx-\frac{\sin(2x)}{4}+\frac{1}{4}x$$
    $$=\frac{1}{8}x+\frac{\sin(4x)}{32}-\frac{\sin(2x)}{4}+\frac{1}{4}x + C$$

*** $\int \sin^n x dx=\frac{n-1}{n}\int sin^{n-2} x dx$
    see [[https://www.coursera.org/learn/calculus1/lecture/FQjH6/what-is-the-integral-of-sin-n-x-dx-in-terms-of-sin-n-2-x-dx][Coursera]]

** Fundamental Theorem of Calculus
   Suppose $f:[a, b]\to \mathbb{R}$ is continuous.

   Let $F$ be the accumulation function, given by
   $$F(x)=\int_{a}^{x}f(t)dt$$
   or
   $$\frac{d}{dx}\int_{a}^{x}f(t)dt=f(x)$$

   Then $F$ is
   - continuous on $[a, b]$
   - differentiable on $(a, b)$
   - $F^\prime(x)=f(x)$
*** $F(b)-F(a)$
    Suppose $f:[a, b]\to \mathbb{R}$ is continuous, and $F$ is an antiderivative of $f$.

    Then
    $$\int_a^bf(x)dx=F(b)-F(a)$$

*** More Details
    $$\frac{d}{db}\int_a^b f(x)dx=f(b)$$
    $$\frac{d}{da}\int_a^b f(x)dx=-f(a)$$
    $$\int_a^b f(x)dx=-\int_b^a f(x)dx$$
** Arc Length
   $$\int\sqrt{dx^2+dy^2} dx=\int\sqrt{1+(\frac{dy}{dx})^2}dx$$
* Series
** $\sum_{i=1}^n i$
   $$\sum_{i=1}^n i=\frac{n(n+1)}{2}$$

** $\sum_{i=1}^n i^2$
   $$\sum_{i=1}^n i^2=\frac{n(n+1)(2n+1)}{6}$$

** $\sum_{i=1}^n i^3$
   Nicomachus's Theorem:
   $$\sum_{i=1}^n i^3=(\sum_{i=1}^n i)^2=\frac{i^2(i+1)^2}{4}$$

* e
** Definition
   1. $e = \lim_{n \to \infty}(1+\frac{1}{n})^n=\lim_{n \to \infty}\sum_{i=0}^nC_i^n1^{n-i}(\frac{1}{n})^i$
   2. $e = \sum_{n=0}^{\infty}\frac{1}{n}$
   3. $\int_1^x\frac{1}{t}dt = 1, then\space x=e$
   4. $\lim_{h\to 0}\frac{x^h-1}{h}=1$
